Bunch further work on declaration correctness

BananasProgram.thy
@@ -25,8 +25,8 @@ fun bind_with_names :: "name \<Rightarrow> (name \<rightharpoonup> type) \<Right
   "bind_with_names n \<Gamma> x = map_option (\<lambda>t. (t, Named n)) (\<Gamma> x)"
 
 inductive typecheck_decl :: "(name \<rightharpoonup> type \<times> type) \<Rightarrow> (name \<rightharpoonup> funct) \<Rightarrow> decl \<Rightarrow> 
-    (name \<rightharpoonup> type \<times> type) \<Rightarrow> (name \<rightharpoonup> funct) \<Rightarrow> bool" (infix " & _ \<Turnstile> _ : _ &" 60) where
-  tcd_type [simp]: "typecheck\<^sub>c cts = (\<Gamma>', F) \<Longrightarrow> 
+    (name \<rightharpoonup> type \<times> type) \<Rightarrow> (name \<rightharpoonup> funct) \<Rightarrow> bool" (infix "& _ \<Turnstile> _ : _ &" 60) where
+  tcd_type [simp]: "typecheck\<^sub>c cts = (\<Gamma>', F) \<Longrightarrow> distinct (map fst cts) \<Longrightarrow>
     \<Gamma> & \<Sigma> \<Turnstile> TypeDecl x cts : \<Gamma> ++ bind_with_names x \<Gamma>' & \<Sigma>(x \<mapsto> F)"
 | tcd_expr [simp]: "\<Gamma> & \<Sigma> \<turnstile> e : t\<^sub>1 \<rightarrow> t\<^sub>2 \<Longrightarrow> \<Gamma> & \<Sigma> \<Turnstile> ExprDecl x e : \<Gamma>(x \<mapsto> (t\<^sub>1, t\<^sub>2)) & \<Sigma>"
 
@@ -37,7 +37,7 @@ inductive typecheck_decls :: "(name \<rightharpoonup> type \<times> type) \<Righ
     (name \<rightharpoonup> type \<times> type) \<Rightarrow> (name \<rightharpoonup> funct) \<Rightarrow> bool" (infix "& _ \<Turnstile> _ :: _ &" 60) where
   tcd_nil [simp]: "\<Gamma> & \<Sigma> \<Turnstile> [] :: \<Gamma> & \<Sigma>"
 | tcd_cons [simp]: "\<Gamma> & \<Sigma> \<Turnstile> \<delta> : \<Gamma>' & \<Sigma>' \<Longrightarrow> binders\<^sub>d \<delta> \<inter> binders \<Lambda> = {} \<Longrightarrow> 
-    \<Gamma>' & \<Sigma> \<Turnstile> \<Lambda> :: \<Gamma>'' & \<Sigma>'' \<Longrightarrow> \<Gamma> & \<Sigma> \<Turnstile> \<delta> # \<Lambda> :: \<Gamma>'' & \<Sigma>''"
+    \<Gamma>' & \<Sigma>' \<Turnstile> \<Lambda> :: \<Gamma>'' & \<Sigma>'' \<Longrightarrow> \<Gamma> & \<Sigma> \<Turnstile> \<delta> # \<Lambda> :: \<Gamma>'' & \<Sigma>''"
 
 inductive_cases [elim]: "\<Gamma> & \<Sigma> \<Turnstile> [] :: \<Gamma>' & \<Sigma>'"
 inductive_cases [elim]: "\<Gamma> & \<Sigma> \<Turnstile> \<delta> # \<Lambda> :: \<Gamma>' & \<Sigma>'"
@@ -66,7 +66,8 @@ primrec is_completed :: "prog \<Rightarrow> bool" where
   "is_completed (Prog \<Lambda> e v) = (e = \<epsilon>)"
 
 inductive evaluate_prog :: "prog \<Rightarrow> prog \<Rightarrow> bool" (infix "\<leadsto>" 60) where
-  ev_prog [simp]: "assemble_context \<Lambda> & \<Sigma> \<turnstile> e \<cdot> v \<leadsto> e' \<cdot> v' \<Longrightarrow> Prog \<Lambda> e v \<leadsto> Prog \<Lambda> e' v'"
+  ev_prog [simp]: "Map.empty & Map.empty \<Turnstile> \<Lambda> :: \<Gamma> & \<Sigma> \<Longrightarrow> 
+    assemble_context \<Lambda> & \<Sigma> \<turnstile> e \<cdot> v \<leadsto> e' \<cdot> v' \<Longrightarrow> Prog \<Lambda> e v \<leadsto> Prog \<Lambda> e' v'"
 
 inductive_cases [elim]: "Prog \<Lambda> e v \<leadsto> \<Pi>"
 
@@ -84,87 +85,89 @@ lemma [simp]: "x \<notin> binders\<^sub>d a \<Longrightarrow> x \<notin> dom (as
 lemma [simp]: "x \<notin> binders \<Lambda> \<Longrightarrow> x \<notin> dom (assemble_context \<Lambda>)"
   by (induction \<Lambda>) simp_all
 
-lemma [simp]: "\<Gamma> & \<Sigma> \<turnstile> e : t\<^sub>1 \<rightarrow> t\<^sub>2 \<Longrightarrow> \<Gamma> & \<Sigma> \<tturnstile> \<Lambda> \<Longrightarrow> x \<notin> dom \<Lambda> \<Longrightarrow> 
-    \<Gamma>(x \<mapsto> (t\<^sub>1, t\<^sub>2)) & \<Sigma> \<tturnstile> \<Lambda>(x \<mapsto> e)"
-  proof (unfold typecheck_context_def, rule, rule, rule, rule)
-    fix y t\<^sub>1' t\<^sub>2'
-    assume A: "\<Gamma> & \<Sigma> \<turnstile> e : t\<^sub>1 \<rightarrow> t\<^sub>2"
-       and B: "\<forall>x t\<^sub>1 t\<^sub>2. \<Gamma> x = Some (t\<^sub>1, t\<^sub>2) \<longrightarrow> (\<exists>e. \<Lambda> x = Some e \<and> \<Gamma> & \<Sigma> \<turnstile> e : t\<^sub>1 \<rightarrow> t\<^sub>2)"
-       and C: "x \<notin> dom \<Lambda>"
-       and D: "(\<Gamma>(x \<mapsto> (t\<^sub>1, t\<^sub>2))) y = Some (t\<^sub>1', t\<^sub>2')"
-    moreover hence E: "x \<notin> dom \<Gamma>" by auto
-    ultimately show "\<exists>e'. (\<Lambda>(x \<mapsto> e)) y = Some e' \<and> \<Gamma>(x \<mapsto> (t\<^sub>1, t\<^sub>2)) & \<Sigma> \<turnstile> e' : t\<^sub>1' \<rightarrow> t\<^sub>2'"
-      proof (cases "x = y")
-      case False
-        with B D obtain e' where "\<Lambda> y = Some e' \<and> \<Gamma> & \<Sigma> \<turnstile> e' : t\<^sub>1' \<rightarrow> t\<^sub>2'" by fastforce
-        with E False show ?thesis by simp
-      qed simp_all
-  qed
-
 lemma [simp]: "bind_with_names x Map.empty = Map.empty"
   by auto
 
 lemma [simp]: "bind_with_names x (\<Gamma>(y \<mapsto> t)) = (bind_with_names x \<Gamma>)(y \<mapsto> (t, Named x))"
   by auto
 
+lemma [simp]: "dom (assemble_context\<^sub>c x cts) = fst ` set cts"
+  proof (induction cts rule: assemble_context\<^sub>c.induct)
+  case (2 n x t cts)
+    hence "dom (assemble_context\<^sub>c n ((x, t) # cts)) = fst ` set ((x, t) # cts)" by simp
+    thus ?case by blast
+  qed simp_all
+
 lemma add_constructors: "typecheck\<^sub>c cts = (\<Gamma>', F) \<Longrightarrow> \<Gamma> & \<Sigma> \<tturnstile> assemble_context \<Lambda> \<Longrightarrow> 
-  fst ` set cts \<inter> binders \<Lambda> = {} \<Longrightarrow> 
-    \<Gamma> ++ bind_with_names x \<Gamma>' & \<Sigma> \<tturnstile> assemble_context \<Lambda> ++ assemble_context\<^sub>c F cts"
+  fst ` set cts \<inter> binders \<Lambda> = {} \<Longrightarrow> x \<notin> dom \<Sigma> \<Longrightarrow> distinct (map fst cts) \<Longrightarrow>
+    \<Gamma> ++ bind_with_names x \<Gamma>' & \<Sigma>(x \<mapsto> F) \<tturnstile> assemble_context \<Lambda> ++ assemble_context\<^sub>c x cts"
   proof (induction cts arbitrary: \<Gamma>' F rule: typecheck\<^sub>c.induct)
-  case (2 y ts cts)
+  case 1
+    hence "\<Gamma> & \<Sigma>(x \<mapsto> K \<zero>) \<tturnstile> assemble_context \<Lambda>" by simp
+    with 1 have "\<Gamma> ++ bind_with_names x \<Gamma>' & \<Sigma>(x \<mapsto> F) \<tturnstile> 
+      assemble_context \<Lambda> ++ assemble_context\<^sub>c x []" by fastforce
+    thus ?case by blast
+  next case (2 y ts cts)
     then obtain \<Gamma>'' Fs where G: "typecheck\<^sub>c cts = (\<Gamma>'', Fs) \<and> \<Gamma>' = \<Gamma>''(y \<mapsto> foldr op \<otimes> ts \<one>) \<and> 
       F = Fs \<Oplus> foldr (\<lambda>t. op \<Otimes> (K t)) ts (K \<one>)" by (auto split: prod.splits)
-    with 2 have "\<Gamma> ++ bind_with_names x \<Gamma>'' \<tturnstile> assemble_context \<Lambda> ++ assemble_context\<^sub>c Fs cts" by fastforce
+    with 2 have "\<Gamma> ++ bind_with_names x \<Gamma>'' & \<Sigma>(x \<mapsto> Fs) \<tturnstile> 
+      assemble_context \<Lambda> ++ assemble_context\<^sub>c x cts" by fastforce
+
 
     let ?t = "foldr op \<otimes> ts \<one>"
     let ?F = "Fs \<Oplus> foldr (\<lambda>t. op \<Otimes> (K t)) ts (K \<one>)"
-    let ?\<Lambda> = "assemble_context \<Lambda>"
+    let ?\<Lambda> = "assemble_context \<Lambda> ++ (map_option (op \<cdot> \<iota>\<^sub>r) \<circ> assemble_context\<^sub>c x cts)"
 
 
-    from 2 have "\<Gamma> \<tturnstile> assemble_context \<Lambda>" by simp
+    from 2 have "\<Gamma> & \<Sigma> \<tturnstile> assemble_context \<Lambda>" by simp
     from 2 have "y \<notin> binders \<Lambda>" by simp
     from 2 have "fst ` set cts \<inter> binders \<Lambda> = {}" by simp
+    from 2 have "y \<notin> fst ` set cts" by simp
+    from 2 have "distinct (map fst cts)" by simp
 
 
-    have X: "(\<Gamma> ++ bind_with_names x \<Gamma>'') \<turnstile> \<prec>\<^bsub>?F\<^esub> \<cdot> \<iota>\<^sub>l : ?t \<rightarrow> Named x" by simp
+    have X: "(\<Gamma> ++ bind_with_names x \<Gamma>'') & \<Sigma>(x \<mapsto> ?F) \<turnstile> \<prec>\<^bsub>x\<^esub> \<cdot> \<iota>\<^sub>l : ?t \<rightarrow> Named x" by simp
 
 
-    have Y: "(\<Gamma> ++ bind_with_names x \<Gamma>'') \<tturnstile> (?\<Lambda> ++ (map_option (op \<cdot> \<iota>\<^sub>r) \<circ> assemble_context\<^sub>c ?F cts))" by simp
+    have Y: "(\<Gamma> ++ bind_with_names x \<Gamma>'') & \<Sigma>(x \<mapsto> ?F) \<tturnstile> ?\<Lambda>" by simp
 
 
-    have "y \<notin> dom (?\<Lambda> ++ (map_option (op \<cdot> \<iota>\<^sub>r) \<circ> assemble_context\<^sub>c ?F cts))" by simp
-    with X Y G have "\<Gamma> ++ bind_with_names x \<Gamma>' \<tturnstile> ?\<Lambda> ++ assemble_context\<^sub>c F ((y, ts) # cts)" by simp
-    thus ?case by blast
-  qed auto
-
-lemma assemble_postpend: "\<Gamma> & \<Sigma> \<Turnstile> \<delta> : \<Gamma>' & \<Sigma>' \<Longrightarrow> \<Gamma> \<tturnstile> assemble_context \<Lambda> \<Longrightarrow> 
-    binders\<^sub>d \<delta> \<inter> binders \<Lambda> = {} \<Longrightarrow> \<Gamma>' \<tturnstile> assemble_context (\<Lambda> @ [\<delta>])"
-  proof (induction \<Gamma> \<Sigma> \<delta> \<Gamma>' \<Sigma>' rule: typecheck_decl.induct)
-  case tcd_type
-    thus ?case using add_constructors by simp
-  next case (tcd_expr \<Gamma> e t\<^sub>1 t\<^sub>2 \<Sigma> x)
-    hence "\<Gamma>(x \<mapsto> (t\<^sub>1, t\<^sub>2)) \<tturnstile> assemble_context (\<Lambda> @ [ExprDecl x e])" by simp
+    from 2 have "y \<notin> dom ?\<Lambda> " by simp
+    with X Y G have "\<Gamma> ++ bind_with_names x \<Gamma>' & \<Sigma>(x \<mapsto> F) \<tturnstile> 
+      assemble_context \<Lambda> ++ assemble_context\<^sub>c x ((y, ts) # cts)" by simp
     thus ?case by blast
   qed
 
-lemma tc_assemble_context [simp]: "\<Gamma> & \<Sigma> \<Turnstile> \<Lambda>' :: \<Gamma>' & \<Sigma>' \<Longrightarrow> \<Gamma> \<tturnstile> assemble_context \<Lambda> \<Longrightarrow> 
-    binders \<Lambda> \<inter> binders \<Lambda>' = {} \<Longrightarrow> \<Gamma>' \<tturnstile> assemble_context \<Lambda> ++ assemble_context \<Lambda>'"
+lemma assemble_postpend: "\<Gamma> & \<Sigma> \<Turnstile> \<delta> : \<Gamma>' & \<Sigma>' \<Longrightarrow> \<Gamma> & \<Sigma> \<tturnstile> assemble_context \<Lambda> \<Longrightarrow> 
+    binders\<^sub>d \<delta> \<inter> binders \<Lambda> = {} \<Longrightarrow> \<Gamma>' & \<Sigma>' \<tturnstile> assemble_context (\<Lambda> @ [\<delta>])"
+  proof (induction \<Gamma> \<Sigma> \<delta> \<Gamma>' \<Sigma>' rule: typecheck_decl.induct)
+  case (tcd_type cts \<Gamma>' F \<Gamma> \<Sigma> x)
+    hence "\<Gamma> ++ bind_with_names x \<Gamma>' & \<Sigma>(x \<mapsto> F) \<tturnstile> assemble_context (\<Lambda> @ [TypeDecl x cts])" 
+      using add_constructors by simp
+    thus ?case by blast
+  next case (tcd_expr \<Gamma> \<Sigma> e t\<^sub>1 t\<^sub>2 x)
+    hence "\<Gamma>(x \<mapsto> (t\<^sub>1, t\<^sub>2)) & \<Sigma> \<tturnstile> assemble_context (\<Lambda> @ [ExprDecl x e])" by simp
+    thus ?case by blast
+  qed
+
+lemma tc_assemble_context [simp]: "\<Gamma> & \<Sigma> \<Turnstile> \<Lambda>' :: \<Gamma>' & \<Sigma>' \<Longrightarrow> \<Gamma> & \<Sigma> \<tturnstile> assemble_context \<Lambda> \<Longrightarrow> 
+    binders \<Lambda> \<inter> binders \<Lambda>' = {} \<Longrightarrow> \<Gamma>' & \<Sigma>' \<tturnstile> assemble_context \<Lambda> ++ assemble_context \<Lambda>'"
   proof (induction \<Gamma> \<Sigma> \<Lambda>' \<Gamma>' \<Sigma>' arbitrary: \<Lambda> rule: typecheck_decls.induct)
   case tcd_nil
     thus ?case by simp
-  next case (tcd_cons \<Gamma> \<Sigma> \<delta> \<Gamma>' \<Sigma>' \<Lambda>' \<Gamma>'')
-    moreover hence "\<Gamma>' \<tturnstile> assemble_context (\<Lambda> @ [\<delta>])" using assemble_postpend by fastforce
+  next case (tcd_cons \<Gamma> \<Sigma> \<delta> \<Gamma>' \<Sigma>' \<Lambda>' \<Gamma>'' \<Sigma>'')
+    moreover hence "\<Gamma>' & \<Sigma>' \<tturnstile> assemble_context (\<Lambda> @ [\<delta>])" using assemble_postpend by fastforce
     moreover from tcd_cons have "binders (\<Lambda> @ [\<delta>]) \<inter> binders \<Lambda>' = {}" by auto
-    ultimately have "\<Gamma>'' \<tturnstile> assemble_context (\<Lambda> @ [\<delta>]) ++ assemble_context \<Lambda>'" by blast
+    ultimately have "\<Gamma>'' & \<Sigma>'' \<tturnstile> assemble_context (\<Lambda> @ [\<delta>]) ++ assemble_context \<Lambda>'" by blast
     thus ?case by simp
   qed
 
-lemma [simp]: "Map.empty & Map.empty \<Turnstile> \<Lambda> :: \<Gamma> & \<Sigma> \<Longrightarrow> \<Gamma> \<tturnstile> assemble_context \<Lambda>"
+lemma [simp]: "Map.empty & Map.empty \<Turnstile> \<Lambda> :: \<Gamma> & \<Sigma> \<Longrightarrow> \<Gamma> & \<Sigma> \<tturnstile> assemble_context \<Lambda>"
   proof -
     assume "Map.empty & Map.empty \<Turnstile> \<Lambda> :: \<Gamma> & \<Sigma>"
-    moreover have "Map.empty \<tturnstile> assemble_context []" by (simp add: typecheck_context_def)
-    ultimately show "\<Gamma> \<tturnstile> assemble_context \<Lambda>" using tc_assemble_context by fastforce
-  qed
+    moreover have "Map.empty & Map.empty \<tturnstile> assemble_context []" by (simp add: typecheck_context_def)
+    ultimately show "\<Gamma> & \<Sigma> \<tturnstile> assemble_context \<Lambda>" using tc_assemble_context by fastforce
+  qed                                                                  
 
 theorem progress [simp]: "\<Pi> \<TTurnstile> \<Gamma> & \<Sigma> : t \<Longrightarrow> is_completed \<Pi> \<or> (\<exists>\<Pi>'. \<Pi> \<leadsto> \<Pi>')"
   proof (induction \<Pi> \<Gamma> \<Sigma> t rule: typecheck_prog.induct)
@@ -172,19 +175,35 @@ theorem progress [simp]: "\<Pi> \<TTurnstile> \<Gamma> & \<Sigma> : t \<Longrigh
     thus ?case 
       proof (cases "e = \<epsilon>")
       case False
-        with tcp_prog obtain e' v' where "assemble_context \<Lambda> \<turnstile> e \<cdot> v \<leadsto> e' \<cdot> v'" by fastforce
-        hence "Prog \<Lambda> e v \<leadsto> Prog \<Lambda> e' v'" by simp
+        with tcp_prog obtain e' v' where "assemble_context \<Lambda> & \<Sigma> \<turnstile> e \<cdot> v \<leadsto> e' \<cdot> v'" by fastforce
+        with tcp_prog have "Prog \<Lambda> e v \<leadsto> Prog \<Lambda> e' v'" by simp
         thus ?thesis by fastforce
       qed simp_all
   qed
 
+lemma [simp]: "\<Gamma> & \<Sigma> \<Turnstile> \<delta> : \<Gamma>\<^sub>1 & \<Sigma>\<^sub>1 \<Longrightarrow> \<Gamma> & \<Sigma> \<Turnstile> \<delta> : \<Gamma>\<^sub>1' & \<Sigma>\<^sub>1' \<Longrightarrow> \<Gamma>\<^sub>1 = \<Gamma>\<^sub>1' \<and> \<Sigma>\<^sub>1 = \<Sigma>\<^sub>1'"
+  proof (induction \<Gamma> \<Sigma> \<delta> \<Gamma>\<^sub>1 \<Sigma>\<^sub>1 rule: typecheck_decl.induct)
+  case (tcd_expr \<Gamma> \<Sigma> e t\<^sub>1 t\<^sub>2 x)
+    thus ?case by simp
+  qed auto
+
+lemma [simp]: "\<Gamma> & \<Sigma> \<Turnstile> \<Lambda> :: \<Gamma>\<^sub>1 & \<Sigma>\<^sub>1 \<Longrightarrow> \<Gamma> & \<Sigma> \<Turnstile> \<Lambda> :: \<Gamma>\<^sub>1' & \<Sigma>\<^sub>1' \<Longrightarrow> \<Gamma>\<^sub>1 = \<Gamma>\<^sub>1' \<and> \<Sigma>\<^sub>1 = \<Sigma>\<^sub>1'"
+  proof (induction \<Gamma> \<Sigma> \<Lambda> \<Gamma>\<^sub>1 \<Sigma>\<^sub>1 rule: typecheck_decls.induct)
+  case (tcd_cons \<Gamma> \<Sigma> \<delta> \<Gamma>\<^sub>2 \<Sigma>\<^sub>2 \<Lambda> \<Gamma>\<^sub>1 \<Sigma>\<^sub>1)
+    moreover then obtain \<Gamma>\<^sub>2' \<Sigma>\<^sub>2' where "(\<Gamma> & \<Sigma> \<Turnstile> \<delta> : \<Gamma>\<^sub>2' & \<Sigma>\<^sub>2') \<and> \<Gamma>\<^sub>2' & \<Sigma>\<^sub>2' \<Turnstile> \<Lambda> :: \<Gamma>\<^sub>1' & \<Sigma>\<^sub>1'" 
+      by fastforce
+    moreover with tcd_cons have "\<Gamma>\<^sub>2 = \<Gamma>\<^sub>2' \<and> \<Sigma>\<^sub>2 = \<Sigma>\<^sub>2'" by fastforce
+    ultimately show ?case by simp
+  qed auto
+
 theorem preservation [simp]: "\<Pi> \<leadsto> \<Pi>' \<Longrightarrow> \<Pi> \<TTurnstile> \<Gamma> & \<Sigma> : t \<Longrightarrow> \<Pi>' \<TTurnstile> \<Gamma> & \<Sigma> : t"
   proof (induction \<Pi> \<Pi>' rule: evaluate_prog.induct)
-  case (ev_prog \<Lambda> e v e' v')
-    then obtain t\<^sub>1 where "(Map.empty & Map.empty \<Turnstile> \<Lambda> :: \<Gamma> & \<Sigma>) \<and> (\<Gamma> \<turnstile> e : t\<^sub>1 \<rightarrow> t) \<and> \<Gamma> \<turnstile> v : t\<^sub>1" 
-      by fastforce
-    moreover with ev_prog obtain t\<^sub>3 where "(\<Gamma> \<turnstile> e' : t\<^sub>3 \<rightarrow> t) \<and> \<Gamma> \<turnstile> v' : t\<^sub>3" by fastforce
-    ultimately show ?case by fastforce
+  case (ev_prog \<Lambda> \<Gamma>' \<Sigma>' e v e' v')
+    moreover then obtain t\<^sub>1 where T: "(Map.empty & Map.empty \<Turnstile> \<Lambda> :: \<Gamma> & \<Sigma>) \<and> 
+      (\<Gamma> & \<Sigma> \<turnstile> e : t\<^sub>1 \<rightarrow> t) \<and> \<Gamma> & \<Sigma> \<turnstile> v : t\<^sub>1" by blast
+    moreover with ev_prog have "\<Gamma> = \<Gamma>' \<and> \<Sigma> = \<Sigma>'" by fastforce
+    ultimately obtain t\<^sub>2 where "(\<Gamma> & \<Sigma> \<turnstile> e' : t\<^sub>2 \<rightarrow> t) \<and> (\<Gamma> & \<Sigma> \<turnstile> v' : t\<^sub>2)" by fastforce
+    with T show ?case by fastforce
   qed
 
 (* big step evaluation *)
@@ -194,21 +213,28 @@ inductive total_evaluate_prog :: "prog \<Rightarrow> val \<Rightarrow> bool" (in
 | ptev_step [simp]: "Prog \<Lambda> e v \<leadsto> Prog \<Lambda> e' v' \<Longrightarrow> Prog \<Lambda> e' v' \<Down> v'' \<Longrightarrow> Prog \<Lambda> e v \<Down> v''"
 
 inductive total_evaluate_prog' :: "prog \<Rightarrow> val \<Rightarrow> bool" (infix "\<Down>\<Down>" 60) where
-  ptev_step' [simp]: "assemble_context \<Lambda> \<turnstile> e \<cdot> v \<Down> v' \<Longrightarrow> Prog \<Lambda> e v \<Down>\<Down> v'"
+  ptev_step' [simp]: "Map.empty & Map.empty \<Turnstile> \<Lambda> :: \<Gamma> & \<Sigma> \<Longrightarrow> 
+    assemble_context \<Lambda> & \<Sigma> \<turnstile> e \<cdot> v \<Down> v' \<Longrightarrow> Prog \<Lambda> e v \<Down>\<Down> v'"
 
 inductive_cases [elim]: "Prog \<Lambda> e v \<Down>\<Down> v'"
 
 lemma [simp]: "\<Pi> \<Down> v = \<Pi> \<Down>\<Down> v"
   proof
-    show "\<Pi> \<Down> v \<Longrightarrow> \<Pi> \<Down>\<Down> v" by (induction \<Pi> v rule: total_evaluate_prog.induct) fastforce+
+    show "\<Pi> \<Down> v \<Longrightarrow> \<Pi> \<Down>\<Down> v" 
+      proof (induction \<Pi> v rule: total_evaluate_prog.induct) 
+      case ptev_base
+        thus ?case by simp
+      next case ptev_step
+        thus ?case by simp
+      qed
   next 
     assume "\<Pi> \<Down>\<Down> v"
     thus "\<Pi> \<Down> v"
       proof (induction \<Pi> v rule: total_evaluate_prog'.induct)
-      case (ptev_step' \<Lambda> e v v')
-        thus ?case 
-          proof (induction "assemble_context \<Lambda>" e v v' rule: total_eval.induct)
-          case (tev_step e v e' v' v'')
+      case (ptev_step' \<Lambda> \<Gamma> \<Sigma> e v v')
+        with ptev_step'(2) show ?case 
+          proof (induction "assemble_context \<Lambda>" \<Sigma> e v v' rule: total_eval.induct)
+          case (tev_step \<Sigma> e v e' v' v'')
             moreover hence "Prog \<Lambda> e v \<leadsto> Prog \<Lambda> e' v'" by simp
             ultimately show ?case by (metis total_evaluate_prog.ptev_step)
           qed simp_all
@@ -217,10 +243,10 @@ lemma [simp]: "\<Pi> \<Down> v = \<Pi> \<Down>\<Down> v"
 
 (* since we are a turing-complete language, total progress is not provable *)
 
-lemma [simp]: "\<Pi> \<Down>\<Down> v \<Longrightarrow> \<Pi> \<TTurnstile> \<Gamma> & \<Sigma> : t \<Longrightarrow> \<Gamma> \<turnstile> v : t"
+lemma [simp]: "\<Pi> \<Down>\<Down> v \<Longrightarrow> \<Pi> \<TTurnstile> \<Gamma> & \<Sigma> : t \<Longrightarrow> \<Gamma> & \<Sigma> \<turnstile> v : t"
   by (induction \<Pi> v rule: total_evaluate_prog'.induct) auto
 
-theorem total_preservation: "\<Pi> \<Down> v \<Longrightarrow> \<Pi> \<TTurnstile> \<Gamma> & \<Sigma> : t \<Longrightarrow> \<Gamma> \<turnstile> v : t"
+theorem total_preservation: "\<Pi> \<Down> v \<Longrightarrow> \<Pi> \<TTurnstile> \<Gamma> & \<Sigma> : t \<Longrightarrow> \<Gamma> & \<Sigma> \<turnstile> v : t"
   by simp
 
 end
